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Abstract

One way to implement higher-order automatic differentiation (AD) is to start with
first-order AD and apply it repeatedly. That works, but for some specific cases, like
evaluating a Taylor series, it can result in combinatorial amounts of redundant com-
putation. This note describes a more efficient method, already known but with a new
presentation, and its implementation in JAX.

1 Introduction

Consider the problem of evaluating the Kth-order Taylor approximation to a function f
around a point x and with an offset v:

f(x+ v) ≈ f(x) + ∂f(x)[v] + 1
2!∂

2f(x)[v, v] + · · ·+ 1
K!∂

Kf(x)[v, . . . , v]. (1)

For a multi-linear function like ∂kf(x) we use square brackets to denote its application to a
list of k separate vectors, like ∂kf(x)[v1, . . . , vk].

A formula like this one involves contracting against many copies of the same perturbation
(tangent) vector v, with terms like

∂kf(x)[v, v, . . . , v︸ ︷︷ ︸
k times

] = ∂kf(x)[v ⊗ v ⊗ · · · ⊗ v︸ ︷︷ ︸
k times

] = ∂kf(x)[v⊗k], (2)

where we abuse notation to apply ∂kf(x) alternatively to a tensor product of vectors.
Compare that to the more generic term

∂kf(x)[v1, v2, . . . , vk] = ∂kf(x)
[⊗

i∈[k] vi
]
, (3)

where v1, . . . , vk may be distinct vectors and [k] := {1, 2, . . . , k}. (Since ∂kf(x) is symmetric
under permuations of its arguments, the tensor product order doesn’t matter.) Our goal is
to find computational savings for the special case of (2) relative to the generic case of (3).
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2 Function composition

Automatic differentiation is about function composition. Consider a composite function
f = g ◦h. We’d like to understand how to express quantities like ∂kf(x)[v1, . . . , vk] in terms
of intermediate quantities ∂nh(x)[· · · ] and the functions ∂mg(x).

Start with k = 1, 2, 3 for concreteness:

∂f(x)[v1] = ∂g(h(x)) [∂h(x)[v1]] . (4)

∂2f(x)[v1, v2] = ∂2g(h(x)) [∂h(x)[v1], ∂h(x)[v2]] + ∂g(h(x))
[
∂2h(x)[v1, v2]

]
. (5)

∂3f(x)[v1, v2, v3] = ∂3g(h(x)) [∂h(x)[v1], ∂h(x)[v2], ∂h(x)[v3]]

+ ∂2g(h(x))
[
∂2h(x)[v1, v3], ∂h(x)[v2]

]
+ ∂2g(h(x))

[
∂h(x)[v1], ∂2h(x)[v2, v3]

]
+ ∂2g(h(x))

[
∂2h(x)[v1, v2], ∂h(x)[v3]

]
+ ∂g(h(x))

[
∂3h(x)[v1, v2, v3]

]
(6)

In Eq. (6) we can see a pattern emerging: each term corresponds to a partition of the
set {1, 2, 3}, with the differentiation order m in each ∂mg(h(x)) and n in each ∂nh(x)[· · · ]
determined by the sizes of the partition and the sizes of the partition elements, respectively.
By induction, in general we have

∂kf(x)[v1, . . . , vk] =
∑

σ∈part([k])

∂|σ|g(h(x))
[⊗

η∈σ ∂
|η|h(x)

[⊗
`∈η v`

]]
, (7)

where part([k]) denotes the set partitions of {1, 2, . . . , k} (so that σ is a set of sets), η ranges
over the partition elements (each a set of integers), and ` ranges over integers.

Now consider when all the perturbation vectors are the same. Going back to the example
in (6), if we set v1 = v2 = v3 = v we can collect the middle three terms:

∂3f(x)[v, v, v] = ∂3g(h(x)) [∂h(x)[v], ∂h(x)[v], ∂h(x)[v]]

+ 3∂2g(h(x))
[
∂h(x)[v], ∂2h(x)[v, v]

]
+ ∂g(h(x))

[
∂3h(x)[v, v, v]

]
. (8)

In general, how many like terms can we collect? It corresponds to this counting problem:
given a set of k elements (the perturbation vectors), in how many ways can we collect them
into m groups (for the arguments to ∂mg(h(x))) using n1 ≥ 0 groups of size 1 (where n1 is
the number of ∂1h(x)[v] terms), n2 groups of size 2 (n2 the number of ∂2h(x)[v, v] terms),
n3 groups of size 3, etc.? The answer is

sym(ν) =

(
k

1, . . . , 1︸ ︷︷ ︸
n1 times

, 2, . . . , 2︸ ︷︷ ︸
n2 times

, . . .

)
1

n1!n2! · · · nk!
, (9)

where ν = (ν1, ν2, . . . , νm) here represents an integer partition of k as a (sorted) tuple of
positive integers with

∑
i νi = k and with ni denoting the number of times i appears in

ν. The first term in (9) is a multinomial coefficient, counting how many ways to collect k
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distinct items into the given numbers and sizes of distinct bins, and the second term corrects
for treating bins of the same size as distinct (thus counting un-distinguished groups).

Putting these pieces together, we have the Faà di Bruno formula,

∂kf(x)[v, . . . , v] =
∑

ν∈part(k)

sym(ν)∂|ν|g(h(x))
[⊗

n∈ν ∂
nh(x)[v⊗n]

]
, (10)

where part(k) denotes the integer partitions of the integer k (rather than set partitions as
in (7)).

3 Composition rule for Taylor series terms

First-order automatic differentiation solves a composition problem: for a function f = g ◦h,
given a pair (z0, z1) = (h(x), ∂h(x)[v]), compute the pair (f(x), ∂f(x)[v]). We solve this
problem using the composition rule

f(x) = g(h(x)) = g(z0), (11)

∂f(x)[v] = ∂g(h(x))[∂h(x)] = ∂g(z0)[z1]. (12)

We implement this rule for every primitive function g and thus can differentiate composite
functions f .

The higher-order analogue is: given a tuple

(z0, z1, z2, . . . , zK) =
(
h(x), ∂h(x)[v], 1

2∂
2h(x)[v, v], . . . 1

K!∂
Kh(x)[v, . . . , v]

)
, (13)

compute the tuple

(w0, w1, w2, . . . , WK) =
(
f(x), ∂f(x)[v], 1

2∂
2f(x)[v, v], . . . 1

K!∂
Kf(x)[v, . . . , v]

)
.

(14)
We can solve this problem using (10), expressing each component as

wk = 1
k!∂

kf(x)[v, . . . , v] =
∑

ν∈part(k)

sym′(ν)∂|ν|g(z0)
[⊗

n∈ν zn
]
, (15)

sym′(ν) =
1

n1!n2! · · · nk!
. (16)

Some of the factorials cancel by including them in the definition of the tuples in (13) and (14).
The Python code implementing (15) may be more legible than the math notation:

def sym(nu):

return prod(fact(count) for _, count in Counter(nu).items())

def prop(derivs, terms):

return [sum(derivs[len(nu)-1]([terms[i-1] for i in nu]) / sym(nu)

for nu in partitions(k))

for k in range(1, len(terms) + 1)]
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Adding and subtracting 1 in places just has to do with off-by-one indexing issues.
The number of integer partitions grows like Θ

(
exp(
√
k)
)
, so direct evaluation of the for-

mula (15) reduces the computational complexity of higher-order differentiation for comput-
ing all the terms in a Taylor series from exponential O

(
2K
)

to subexponential O
(

exp(
√
K)
)
,

but not further. However, the combinatorial structure of the formula enables more efficient
evaluation via a recurrence.

4 Reducing complexity for common primitives to O(K2)

One simple case where we can reduce the complexity in (15) is when the function g has some
derivatives that are zero. For example, when g is linear (or bilinear) so that ∂kg(x) ≡ 0
for k > 1, then the complexity of evaluating (15) for k = 1, 2, . . . ,K is O

(
K
)
. This case

handles all the common bilinear operations on arrays (contracion, convolution, etc.).
What about element-wise unary nonlinear functions, like exp and sin, which have no zero

derivatives? For these we can exploit the fact that they satisfy first-order linear ordinary
differential equations (ODEs). The basic idea is that while Eq. (15) generates a system of
equations, expressing each wk in terms of zj≤k, the expressions in zj≤k get large. However,
if g satisfies an ODE, that produces additional constraints on the Taylor coefficients. We
can use those constraints to write equations for wk in terms of both zj≤k and wi<k.

For example, g = exp has no zero derivatives but satisfies g′(y) = g(y), where we write
g′(y) = ∂g(y)[1] for the scalar (element-wise) case. To see the constraints among the Taylor
series coefficients, we substitute the ODE in the chain rule statement

f ′(x) = g′(h(x))h′(x) = g(h(x))h′(x) = f(x)h′(x). (17)

Substituting the Taylor expansions

f(x) =

∞∑
k=0

wkx
k, g(x) =

∞∑
k=0

zkx
k, (18)

we get
∞∑
k=1

k wk x
k−1 =

( ∞∑
k=0

wk x
k

)( ∞∑
k=1

k zk x
k−1

)
, (19)

and equating coefficients we get

k wk =

k∑
`=1

`wk−` z`, k = 1, 2, . . . ,K. (20)

With these equations we can solve for the wk in time O(K2). These equations hold true
element-wise for the vector case because we can use the expansions

f(x+ tv) =

∞∑
k=0

1
k!∂

kf(x)[v⊗k]tk =

∞∑
k=0

wkt
k, g(x+ tv) =

∞∑
k=0

1
k!∂

kg(x)[v⊗k]tk =

∞∑
k=0

zkt
k.

Slightly more generally, Proposition 13.1 in Griewank and Walter follows this reasoning
to provide the result that if g satisfies the first-order linear ODE

b(y)g′(y) = a(y)g(y) + c(y), (21)
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then the coefficients satisfy

k wk =
1

b0

 k∑
j=1

j (ck−jek−j) zj −
k−1∑
j=1

j bk−jwj

 , k = 1, 2, . . . ,K, (22)

ek =

k∑
j=0

ajwk−j , k = 1, 2, . . . ,K − 1. (23)
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